pulse/lib/pulse/core/PulseCore.Heap2.fst
@@ -548,6 +548,7 @@ let lift_erased
   refined_pre_action_as_action g
 
 let core_ghost_ref = erased H.core_ref
+let core_ghost_ref_eq x y = H.core_ref_eq (reveal x) (reveal y)
 let ghost_pts_to meta #a #p r v = llift GHOST (H.pts_to meta #a #p r v)
 let ghost_free_above_addr h addr = H.free_above_addr h.ghost addr
 
